syntax: improve strict polopt roundtrip reliability

lib/OpenScopPrinter.ml
@@ -123,6 +123,7 @@ let rec arr_expr_str arr_expr =
       | OpenScop.AInt z -> Camlcoq.Z.to_string z
       | OpenScop.AVar id -> Camlcoq.camlstring_of_coqstring id
       | OpenScop.AFloat f -> Float.to_string (Camlcoq.camlfloat_of_coqfloat f)
+      | OpenScop.AFloatLiteral f -> Camlcoq.camlstring_of_coqstring f
     )  
   | OpenScop.ArrAccessAtom (arr_access) -> 
       arr_access_str arr_access 
@@ -138,6 +139,10 @@ let rec arr_expr_str arr_expr =
     (arr_expr_str arr_expr1) ^ " < " ^ (arr_expr_str arr_expr2)
   | OpenScop.ArrLe (arr_expr1, arr_expr2) -> 
     (arr_expr_str arr_expr1) ^ " <= " ^ (arr_expr_str arr_expr2)
+  | OpenScop.ArrEq (arr_expr1, arr_expr2) ->
+    (arr_expr_str arr_expr1) ^ " == " ^ (arr_expr_str arr_expr2)
+  | OpenScop.ArrAnd (arr_expr1, arr_expr2) ->
+    (arr_expr_str arr_expr1) ^ " && " ^ (arr_expr_str arr_expr2)
   | OpenScop.ArrCond (arr_expr1, arr_expr2, arr_expr3) -> 
     (arr_expr_str arr_expr1) ^ " ? " ^ (arr_expr_str arr_expr2) ^ " : " ^ (arr_expr_str arr_expr3)
   | OpenScop.ArrCall (id, arr_exprs) -> 
